\setcounter{equation}{0}

\question \textgreek{Αρχικά έχουμε ότι: }

\begin{center}
        
\begin{align*}
    &\int_{-1}^{1}(1-x)^\kappa dx = \left[\frac{(1-x)^{\kappa+1}}{\kappa+1}\right]_{-1}^{1} = -\frac{2^{\kappa+1}}{\kappa+1}\\
    \implies &\lim_{\kappa\to0}\int_{-1}^{1}(1-x)^\kappa dx = \lim_{\kappa\to0}-\frac{2^{\kappa+1}}{\kappa+1} = \lim_{\kappa\to0}-\frac{2^{\kappa+1}}{\kappa+1}
    = \lim_{\kappa\to0}-\frac{e^{(\kappa+1)ln2}}{\kappa+1}\\
    \overset{\mathrm{u=\kappa+1}}{=\joinrel=\joinrel=} & \lim_{u\to0}-\frac{e^{uln2}}{u} = (-1)\cdot \pm \infty
\end{align*}
        
\textgreek{Άρα το όριο δεν υπάρχει.\\ Παίρνοντας το όριο στο $+\infty$ έχουμε: }
        
\begin{align*}
    \lim_{\kappa\to+\infty}-\frac{2^{\kappa+1}}{\kappa+1} = &\lim_{\kappa\to+\infty}-\frac{2^{\kappa+1}}{\kappa+1}
    = \lim_{\kappa\to+\infty}-\frac{e^{(\kappa+1)ln2}}{\kappa+1}
    \overset{\mathrm{u=\kappa+1}}{=\joinrel=\joinrel=}\lim_{u\to+\infty}-\frac{e^{uln2}}{u}\\
    \underset{\mathrm{DLH}}{\overset{\left(\frac{\infty}{\infty}\right)}{=\joinrel=}}&\lim_{u\to+\infty}-\frac{ln2\cdot e^{uln2}}{1} = -ln2 \cdot (+\infty) = -\infty
\end{align*}
        
\end{center}