\setcounter{page}{1}
\setcounter{equation}{0}

\question

\begin{center}
\begin{proof}[\unskip\nopunct]
\begin{align}
    \notag
    &\int_{\alpha}^{\beta}f(x)dx + \int_{\gamma}^{\delta}f^{-1}(x)dx = \beta\cdot\delta - \alpha\cdot\gamma\notag
    \implies \int_{\alpha}^{\beta}f(x)dx + \int_{\gamma}^{\delta}f^{-1}(x)dx = \left[xf(x)\right]_{\alpha}^{\beta}\\
    &\implies \int_{\alpha}^{\beta}f(x)dx = \left[xf(x)\right]_{\alpha}^{\beta} - \int_{\gamma}^{\delta}f^{-1}(x)dx
\end{align}
\textgreek{Θέτοντας $u=f^{-1}(x)\implies x=f(u) \implies dx=f'(u)du$ και $u_1 = f^{-1}(\gamma) = \alpha$, $u_2 = f^{-1}(\delta) = \beta$}
\begin{align}
    \int_{\gamma}^{\delta}f^{-1}(x)dx = \int_{\alpha}^{\beta}uf'(u)du = \int_{\alpha}^{\beta}xf'(x)dx
\end{align}

\textgreek{Οπότε θα έχουμε: }
\begin{align*}
    \underset{\mathrm{(2)}}{\overset{\mathrm{(1)}}{\implies}} \implies \int_{\alpha}^{\beta}f(x)dx = \left[xf(x)\right]_{\alpha}^{\beta} - \int_{\alpha}^{\beta}xf'(x)dx
\end{align*}
\textgreek{Το οποίο ισχύει καθώς είναι ο ορισμός της ολοκλήρωσης κατα παράγοντες.}
\end{proof}

\end{center}