\setcounter{equation}{0}

\question  

\begin{align*}
    &y^2 - 2y -x^2 + 1 = 0
    \implies y^2 - 2y -x^2 + 1 -x + x = 0\\
    \implies &y^2 - 2y -x^2 + 1 -x + x  -xy + xy = 0\\
    \implies &y^2 +xy -y -xy -x^2 + x -y -x + 1 = 0\\
    \implies &(y-x-1)(y+x-1)=0
\end{align*}
\begin{center}
\textgreek{Οπότε οι ευθείες είναι: $(\varepsilon_1): y = x + 1$ και $(\varepsilon_2): y = -x + 1$}
        
\begin{tikzpicture}
    \begin{axis}[
        samples=100,grid=major,
        width=10cm,
        axis lines = middle,
        xmin=-1.5, xmax=1.5, ymin=-0.5, ymax=2,
    ]
    \addplot[blue] (x,x+1);
    \addplot[red] (x,-x+1);
    \addplot[name path=e1, red, domain=0:1] (x,-x+1);
    \addplot[name path=e2, blue, domain=-1:0] (x,x+1);
    \path[name path=axis] (axis cs:-1,0) -- (axis cs:1,0);
    \addplot [
        thick,
        color=blue,
        fill=blue,
        fill opacity=0.05
    ]
    fill between[
        of=e2 and axis,
        soft clip={domain=-1:1},
    ];
    \node [rotate=0] at (axis cs:  .25,  .25) {\Huge$\Omega$};
    \end{axis}
\end{tikzpicture}
      
\textgreek{Οπότε έχουμε ότι:}
      
\begin{equation*}
    E(\Omega) = \frac{1}{2}2\cdot 1 = 1
\end{equation*}

\end{center}